hax-lib/proof-libs/fstar/rust_primitives/Rust_primitives.Slice.fsti
@@ -18,6 +18,41 @@ let slice_copy_within (#v_T: Type0) (s: t_Slice v_T)
   Seq.append (Seq.slice s 0 (v dest))
     (Seq.append (Seq.slice s (v start) (v end_))
       (Seq.slice s (v dest + (v end_ - v start)) (Seq.length s)))
+let slice_chunk_bound_lemma (len: nat) (n: pos) (i: nat)
+  : Lemma (requires i < len / n) (ensures n * (i + 1) <= len)
+  = FStar.Math.Lemmas.lemma_mult_le_left n (i + 1) (len / n);
+    FStar.Math.Lemmas.lemma_div_mod len n
+
+let slice_as_chunks (#t: Type0) (n: usize {v n > 0}) (s: t_Slice t)
+  : res: (t_Slice (t_Array t n) & t_Slice t) {
+      let (chunks, rest) = res in
+      Seq.length chunks == Seq.length s / v n /\
+      (forall (i: nat). i < Seq.length chunks ==>
+         (Seq.index chunks i <: Seq.seq t) == Seq.slice s (v n * i) (v n * (i + 1))) /\
+      rest == Seq.slice s (v n * (Seq.length s / v n)) (Seq.length s) /\
+      Seq.length rest == Seq.length s % v n } =
+  let k = Seq.length s / v n in
+  FStar.Math.Lemmas.lemma_div_mod (Seq.length s) (v n);
+  Seq.init #(t_Array t n) k (fun i -> slice_chunk_bound_lemma (Seq.length s) (v n) i;
+                       Seq.slice s (v n * i) (v n * (i + 1))),
+  Seq.slice s (v n * k) (Seq.length s)
+
+let slice_as_rchunks (#t: Type0) (n: usize {v n > 0}) (s: t_Slice t)
+  : res: (t_Slice t & t_Slice (t_Array t n)) {
+      let (rest, chunks) = res in
+      let r = Seq.length s % v n in
+      rest == Seq.slice s 0 r /\
+      Seq.length rest == r /\
+      Seq.length chunks == Seq.length s / v n /\
+      (forall (i: nat). i < Seq.length chunks ==>
+         (Seq.index chunks i <: Seq.seq t) == Seq.slice s (r + v n * i) (r + v n * (i + 1))) } =
+  let k = Seq.length s / v n in
+  let r = Seq.length s % v n in
+  FStar.Math.Lemmas.lemma_div_mod (Seq.length s) (v n);
+  Seq.slice s 0 r,
+  Seq.init #(t_Array t n) k (fun i -> slice_chunk_bound_lemma (Seq.length s) (v n) i;
+                       Seq.slice s (r + v n * i) (r + v n * (i + 1)))
+
 val array_map (#t: Type) (#u: Type) (l: usize) (#ft: Type)
   (s: t_Array t l) (f: t -> u): res: t_Array u l {forall i. Seq.index res i == f (Seq.index s i)}
 let array_as_slice (#t: Type) (l: usize) (s: t_Array t l): t_Slice t =
